

6.1.1)

$$T_1\left(\begin{bmatrix} x \\ y \end{bmatrix}\right) = \begin{bmatrix} 2x+y \\ x-2y \\ -x-y \end{bmatrix} = x \begin{bmatrix} 2 \\ 1 \\ -1 \end{bmatrix} + y \begin{bmatrix} 1 \\ -2 \\ -1 \end{bmatrix} \quad A = \begin{bmatrix} 2 & 1 \\ 1 & -2 \\ -1 & -1 \end{bmatrix} \quad \text{linear} \checkmark$$

$$T_2\left(\begin{bmatrix} x \\ y \\ z \end{bmatrix}\right) = \begin{bmatrix} x+y^2 \\ (x+y)z \\ 0 \end{bmatrix} \quad \begin{array}{l} u+v = (0, 2, 0), T_2(u+v) = (0+4, 0+2 \cdot 0, 0) = (4, 0, 0) \\ T_2(u) = (1, 0, 0), T_2(v) = (1, 0, 0) \quad T_2(u) + T_2(v) = (2, 0, 0) \end{array}$$

Not Linear

$$T_3\left(\begin{bmatrix} x \\ y \\ z \end{bmatrix}\right) = \begin{bmatrix} 0 \\ 0 \\ 0 \end{bmatrix} \quad T_3(u+v) = 0+0+0 = T_3(u) + T_3(v) \quad \text{Linear}$$

$T_1 = \text{linear} \quad T_3 = \text{linear} \quad T_2 = \text{not linear}$

6.2.1) a)

$$(T(v))_k = \begin{cases} v_k & \text{if } k \neq j \\ bv_j & \text{if } k = j \end{cases}$$

$$\text{For } k \neq j, (T(u+v))_k = u_k + v_k = (T(u))_k + (T(v))_k$$

$$\text{For } k = j, (T(u+v))_j = b(u_j + v_j) = bu_j + bv_j = (T(u))_j + (T(v))_j$$

T is linear

$$A = I + (b-1)e_j e_j^T \quad A = \begin{bmatrix} 1 & 0 & 0 \\ 0 & b & 0 \\ 0 & 0 & 1 \end{bmatrix}$$

b)

$$\text{For } k \neq i, T(u+v)_k = u_k + v_k = T(u)_k + T(v)_k$$

$$\text{For } k = i, T(u+v)_i = (u_i + v_i) + b(u_j + v_j) = (u_i + bu_j) + (v_i + bv_j) = T(u)_i + T(v)_i$$

T is linear

$$A = I + be_i e_i^T$$

$$A = \begin{bmatrix} 1 & 0 & 0 \\ b & 1 & 0 \\ 0 & 0 & 1 \end{bmatrix}$$

$$c) T(v)_k = v_k \text{ if } k \neq i, j, T(v)_i = v_j, T(v)_j = v_i$$

$$A_{kl} = \begin{cases} \delta_{kl} & \text{if } l \neq i, j \\ 1 & \text{if } (k, l) = (i, j) \text{ or } (k, l) = (j, i) \\ 0 & \text{if } (k, l) = (i, i) \text{ or } (j, j) \text{ when swapped} \end{cases}$$

$$A = \begin{bmatrix} 0 & 0 & 1 \\ 0 & 1 & 0 \\ 1 & 0 & 0 \end{bmatrix} \quad Ae_i = e_j, Ae_j = e_i, Ae_k = e_k$$

$$6.2.3) \quad u_1 = \begin{bmatrix} 1 \\ 2 \\ -6 \end{bmatrix}, u_2 = \begin{bmatrix} -1 \\ -1 \\ 5 \end{bmatrix}, u_3 = \begin{bmatrix} 0 \\ -1 \\ 2 \end{bmatrix}$$

$$v_1 = \begin{bmatrix} 5 \\ 1 \\ 3 \end{bmatrix}, v_2 = \begin{bmatrix} 1 \\ 1 \\ 5 \end{bmatrix}, v_3 = \begin{bmatrix} 5 \\ 3 \\ 2 \end{bmatrix}$$

$$A = \begin{bmatrix} 1 & -1 & 0 \\ 2 & -1 & -1 \\ -6 & 5 & 2 \end{bmatrix} \quad B = \begin{bmatrix} 5 & 1 & 5 \\ 1 & 1 & 3 \\ 3 & 5 & -2 \end{bmatrix}$$

$$\det(A) = \det \begin{bmatrix} 1 & -1 \\ 5 & 2 \end{bmatrix} - (-1) \det \begin{bmatrix} 2 & -1 \\ -6 & 2 \end{bmatrix}$$

$$1 \cdot (-1(2) - (-1)(5)) + 1((2)(2) - (-1)(6))$$

$$3 - 2 = 1$$

$$\left[\begin{array}{ccc|ccc} 1 & -1 & 0 & 1 & 0 & 0 \\ 2 & -1 & -1 & 0 & 1 & 0 \\ -6 & 5 & 2 & 0 & 0 & 1 \end{array} \right] \begin{array}{l} R_2 - 2R_1 \\ R_3 + 6R_1 \end{array} \left[\begin{array}{ccc|ccc} 1 & -1 & 0 & 1 & 0 & 0 \\ 0 & 1 & -1 & -2 & 1 & 0 \\ 0 & -1 & 2 & 6 & 0 & 1 \end{array} \right]$$

$$\begin{array}{l} R_3 + R_2 \\ R_1 + R_2 \end{array} \left[\begin{array}{ccc|ccc} 1 & -1 & 0 & 1 & 0 & 0 \\ 0 & 1 & -1 & -2 & 1 & 0 \\ 0 & 0 & 1 & 4 & 1 & 1 \end{array} \right] \begin{array}{l} R_1 + R_3 \\ R_2 + R_3 \end{array} \left[\begin{array}{ccc|ccc} 1 & 0 & 0 & 5 & 1 & 1 \\ 0 & 1 & 0 & 2 & 2 & 1 \\ 0 & 0 & 1 & 4 & 1 & 1 \end{array} \right] \quad A^{-1} = \begin{bmatrix} 5 & 1 & 1 \\ 2 & 2 & 1 \\ 4 & 1 & 1 \end{bmatrix}$$

$$BA^{-1} = \begin{bmatrix} 5 & 1 & 5 \\ 1 & 1 & 3 \\ 3 & 5 & -2 \end{bmatrix} \begin{bmatrix} 5 & 1 & 1 \\ 2 & 2 & 1 \\ 4 & 1 & 1 \end{bmatrix} = \boxed{\begin{bmatrix} 37 & 17 & 11 \\ 17 & 7 & 5 \\ 11 & 14 & 6 \end{bmatrix}}$$

$$6.3.1) R(\theta) = \begin{bmatrix} \cos \theta & -\sin \theta \\ \sin \theta & \cos \theta \end{bmatrix} \quad \theta = \pi/3$$

$$R(\frac{\pi}{3}) = \begin{bmatrix} 1/2 & -\frac{\sqrt{3}}{2} \\ \frac{\sqrt{3}}{2} & 1/2 \end{bmatrix}$$

$$6.4.1) R_x = \begin{bmatrix} 1 & 0 \\ 0 & -1 \end{bmatrix} \quad R_y = \begin{bmatrix} -1 & 0 \\ 0 & 1 \end{bmatrix}$$

$$R_y R_x = \begin{bmatrix} -1 & 0 \\ 0 & 1 \end{bmatrix} \begin{bmatrix} 1 & 0 \\ 0 & -1 \end{bmatrix} = \begin{bmatrix} -1 & 0 \\ 0 & -1 \end{bmatrix}$$

$$6.4.3) R_{\pi/6} = \begin{bmatrix} \cos \frac{\pi}{6} & -\sin \frac{\pi}{6} \\ \sin \frac{\pi}{6} & \cos \frac{\pi}{6} \end{bmatrix} = \begin{bmatrix} \frac{\sqrt{3}}{2} & -1/2 \\ 1/2 & \sqrt{3}/2 \end{bmatrix}$$

$$F_y F_x = \begin{bmatrix} -1 & 0 \\ 0 & -1 \end{bmatrix} \quad M = (F_y F_x) R_{\pi/6} = \begin{bmatrix} -1 & 0 \\ 0 & -1 \end{bmatrix} \begin{bmatrix} \frac{\sqrt{3}}{2} & -1/2 \\ 1/2 & \sqrt{3}/2 \end{bmatrix} = \begin{bmatrix} -\frac{\sqrt{3}}{2} & 1/2 \\ -1/2 & -\sqrt{3}/2 \end{bmatrix}$$

$$6.4.7) A_v = \begin{bmatrix} 3 & 1 \\ -1 & 2 \end{bmatrix} \begin{bmatrix} 2 \\ -1 \end{bmatrix} = \begin{bmatrix} 3 \cdot 2 + 1 \cdot (-1) \\ -1 \cdot 2 + 2 \cdot (-1) \end{bmatrix} = \begin{bmatrix} 5 \\ -4 \end{bmatrix}$$

$$B \cdot A_v = \begin{bmatrix} 0 & -2 \\ 4 & 2 \end{bmatrix} \begin{bmatrix} 5 \\ -4 \end{bmatrix} = \begin{bmatrix} 0 \cdot 5 + (-2) \cdot (-4) \\ 4 \cdot 5 + 2 \cdot (-4) \end{bmatrix} = \begin{bmatrix} 8 \\ 12 \end{bmatrix}$$

$$(S \circ T)(v) = \begin{bmatrix} 8 \\ 12 \end{bmatrix}$$

$$6.4.10)$$

$$\det(A) = (2)(2) - (1)(5) = -1$$

$$A^{-1} = \frac{1}{\det(A)} \begin{bmatrix} d & -b \\ -c & a \end{bmatrix} = \frac{1}{-1} \begin{bmatrix} 2 & -1 \\ -5 & 2 \end{bmatrix}$$

$$T^{-1} = \begin{bmatrix} -2 & 1 \\ 5 & -2 \end{bmatrix}$$